
\documentclass[10pt,fleqn]{report}
\usepackage[vcentering]{geometry}
\geometry{papersize={14in,11in},total={13in,10in}}

\pagestyle{empty}
\usepackage[latin1]{inputenc}
\usepackage{amsmath}
\usepackage{amsfonts}
\usepackage{amssymb}
\usepackage{amsbsy}
\usepackage{tensor}
\usepackage{listings}
\usepackage{color}
\usepackage{xcolor}
\usepackage{bm}
\usepackage{breqn}
\definecolor{gray}{rgb}{0.95,0.95,0.95}
\setlength{\parindent}{0pt}
\newcommand{\eb}{\boldsymbol{e}}
\usepackage{float}
\floatstyle{plain} % optionally change the style of the new float
\newfloat{Code}{H}{myc}
\lstloadlanguages{Python}

\DeclareMathOperator{\Tr}{Tr}
\DeclareMathOperator{\Adj}{Adj}
\newcommand{\bfrac}[2]{\displaystyle\frac{#1}{#2}}
\newcommand{\lp}{\left (}
\newcommand{\rp}{\right )}
\newcommand{\paren}[1]{\lp {#1} \rp}
\newcommand{\half}{\frac{1}{2}}
\newcommand{\llt}{\left <}
\newcommand{\rgt}{\right >}
\newcommand{\abs}[1]{\left |{#1}\right | }
\newcommand{\pdiff}[2]{\bfrac{\partial {#1}}{\partial {#2}}}
\newcommand{\npdiff}[3]{\bfrac{\partial^{#3} {#1}}{\partial {#2}^{#3}}}
\newcommand{\lbrc}{\left \{}
\newcommand{\rbrc}{\right \]}
\newcommand{\lbrk}{\left \[}
\newcommand{\rbrk}{\right \}}
\newcommand{\W}{\wedge}
\newcommand{\prm}[1]{{#1}'}
\newcommand{\ddt}[1]{\bfrac{d{#1}}{dt}}
\newcommand{\R}{\dagger}
\newcommand{\deriv}[3]{\bfrac{d^{#3}#1}{d{#2}^{#3}}}
\newcommand{\grd}[1]{\left < {#1} \right >}
\newcommand{\f}[2]{{#1}\lp {#2} \rp}
\newcommand{\eval}[2]{\left . {#1} \right |_{#2}}
\newcommand{\bs}[1]{\boldsymbol{#1}}
\newcommand{\es}[1]{\boldsymbol{e}_{#1}}
\newcommand{\eS}[1]{\boldsymbol{e}^{#1}}
\newcommand{\grade}[2]{\left < {#1} \right >_{#2}}
\newcommand{\lc}{\rfloor}
\newcommand{\rc}{\lfloor}
\newcommand{\T}[1]{\text{#1}}
\newcommand{\lop}[1]{\overleftarrow{#1}}
\newcommand{\rop}[1]{\overrightarrow{#1}}
\newcommand{\ldot}{\lfloor}
\newcommand{\rdot}{\rfloor}

%MacDonald LaTeX macros

\newcommand   {\thalf}    {\textstyle \frac{1}{2}}
\newcommand   {\tthird}   {\textstyle \frac{1}{3}}
\newcommand   {\tquarter} {\textstyle \frac{1}{4}}
\newcommand   {\tsixth}   {\textstyle \frac{1}{6}}

\newcommand   {\RE}       {\mathbb{R}}
\newcommand   {\GA}       {\mathbb{G}}
\newcommand   {\inner}    {\mathbin{\pmb{\cdot}}}
\renewcommand {\outer}    {\mathbin{\wedge}}
\newcommand   {\cross}    {\mathbin{\times}}
\newcommand   {\meet}     {\mathbin{{\,\vee\;}}}
\renewcommand {\iff}              {\Leftrightarrow}
\renewcommand {\impliedby}{\Leftarrow}
\renewcommand {\implies}  {\Rightarrow}
\newcommand   {\perpc}    {\perp}  % Orthogonal complement
\newcommand   {\perpm}    {*}  % Dual of multivector
\newcommand   {\del}      {\mathbf{\nabla}}  %{\boldsymbol\nabla\!}
\newcommand   {\mpart}[2]{\left\langle\, #1 \,\right\rangle_{#2}} % AMS has a \part
\newcommand   {\spart}[1]{\mpart{#1}{0}}
\newcommand   {\ds}       {\displaystyle}
\newcommand   {\os}       {\overset}
\newcommand   {\galgebra} {\mbox{$\mathcal{G\!A}$\hspace{.01in}lgebra}}
\newcommand   {\latex}    {\LaTeX}
\begin{document}\begin{lstlisting}[language=Python,showspaces=false,showstringspaces=false,backgroundcolor=\color{gray},frame=single]
def Product_of_Rotors():
    Print_Function()
    (na,nb,nm,alpha,th,th_a,th_b) = symbols('n_a n_b n_m alpha theta theta_a theta_b',\
                                    real = True)
    g = [[na, 0, alpha],[0, nm, 0],[alpha, 0, nb]] #metric tensor
    """
    Values of metric tensor components
    [na,nm,nb] = [+1/-1,+1/-1,+1/-1]  alpha = ea|eb
    """
    (g3d, ea, em, eb) = Ga.build('e_a e_m e_b', g=g)
    print('g =',g3d.g)
    print(r'n_{a} = \bm{e}_{a}^{2}\;\;n_{b} = \bm{e}_{b}^{2}\;\;n_{m} = \bm{e}_{m}^{2}'+\
        r'\;\;\alpha = \bm{e}_{a}\cdot\bm{e}_{b}')
    (ca,cb,sa,sb) = symbols('c_a c_b s_a s_b',real=True)
    Ra = ca + sa*ea*em  # Rotor for ea^em plane
    Rb = cb + sb*em*eb  # Rotor for em^eb plane
    print(r'\mbox{Rotor in }\bm{e}_{a}\bm{e}_{m}\mbox{ plane } R_{a} =',Ra)
    print(r'\mbox{Rotor in }\bm{e}_{m}\bm{e}_{b}\mbox{ plane } R_{b} =',Rb)
    Rab = Ra*Rb  # Compound Rotor
    """
    Show that compound rotor is scalar plus bivector
    """
    print(r'R_{a}R_{b} = S+\bm{B} =', Rab)
    Rab2 = Rab.get_grade(2)
    print(r'\bm{B} =',Rab2)
    Rab2sq = Rab2*Rab2  # Square of compound rotor bivector part
    Ssq = (Rab.scalar())**2  # Square of compound rotor scalar part
    Bsq =  Rab2sq.scalar()
    print(r'S^{2} =',Ssq)
    print(r'\bm{B}^{2} =',Bsq)
    Dsq = (Ssq-Bsq).expand().simplify()
    print('S^{2}-B^{2} =', Dsq)
    Dsq = Dsq.subs(nm**2,S(1))  # (e_m)**4 = 1
    print('S^{2}-B^{2} =', Dsq)
    Cases = [S(-1),S(1)]  # -1/+1 squares for each basis vector
    print(r'\T{Consider all combinations of} \bm{e}_{a}^{2}, \bm{e}_{b}^{2}'+\
          r' \T{and} \bm{e}_{m}^2:')
    for Na in Cases:
        for Nb in Cases:
            for Nm in Cases:
                Ba_sq = -Na*Nm
                Bb_sq = -Nb*Nm
                if Ba_sq < 0:
                    Ca_th = cos(th_a)
                    Sa_th = sin(th_a)
                else:
                    Ca_th = cosh(th_a)
                    Sa_th = sinh(th_a)
                if Bb_sq < 0:
                    Cb_th = cos(th_b)
                    Sb_th = sin(th_b)
                else:
                    Cb_th = cosh(th_b)
                    Sb_th = sinh(th_b)
                print(r'\left [ \bm{e}_{a}^{2},\bm{e}_{b}^{2},\bm{e}_{m}^2\right ] =',\
                      [Na,Nb,Nm])
                Dsq_tmp = Dsq.subs({ca:Ca_th,sa:Sa_th,cb:Cb_th,sb:Sb_th,na:Na,nb:Nb,nm:Nm})
                print(r'S^{2}-\bm{B}^{2} =',Dsq_tmp,' =',trigsimp(Dsq_tmp))
    print(r'\T{Thus we have shown that }R_{a}R_{b} = S+\bm{D} = e^{\bm{C}} \T{where} \bm{C}'+\
          r' \T{is a bivector blade.}')
    return

\end{lstlisting}
\T{Code Output:}
\begin{equation} g =  \left [ \begin{array}{ccc} n_{a} & 0 & \alpha   \\ 0 & n_{m} & 0  \\ \alpha  & 0 & n_{b}  \end{array}\right ]  \nonumber\end{equation}
\begin{equation} n_{a} = \bm{e}_{a}^{2}\;\;n_{b} = \bm{e}_{b}^{2}\;\;n_{m} = \bm{e}_{m}^{2}\;\;\alpha = \bm{e}_{a}\cdot\bm{e}_{b} \nonumber\end{equation}
\begin{equation} \mbox{Rotor in }\bm{e}_{a}\bm{e}_{m}\mbox{ plane } R_{a} = c_{a}  + s_{a} \boldsymbol{e}_{a}\wedge \boldsymbol{e}_{m} \nonumber\end{equation}
\begin{equation} \mbox{Rotor in }\bm{e}_{m}\bm{e}_{b}\mbox{ plane } R_{b} = c_{b}  + s_{b} \boldsymbol{e}_{m}\wedge \boldsymbol{e}_{b} \nonumber\end{equation}
\begin{equation} R_{a}R_{b} = S+\bm{B} = \left ( \alpha  n_{m} s_{a} s_{b} + c_{a} c_{b}\right )  + c_{b} s_{a} \boldsymbol{e}_{a}\wedge \boldsymbol{e}_{m} + n_{m} s_{a} s_{b} \boldsymbol{e}_{a}\wedge \boldsymbol{e}_{b} + c_{a} s_{b} \boldsymbol{e}_{m}\wedge \boldsymbol{e}_{b} \nonumber\end{equation}
\begin{equation} \bm{B} = c_{b} s_{a} \boldsymbol{e}_{a}\wedge \boldsymbol{e}_{m} + n_{m} s_{a} s_{b} \boldsymbol{e}_{a}\wedge \boldsymbol{e}_{b} + c_{a} s_{b} \boldsymbol{e}_{m}\wedge \boldsymbol{e}_{b} \nonumber\end{equation}
\begin{equation} S^{2} = \left(\alpha  n_{m} s_{a} s_{b} + c_{a} c_{b}\right)^{2} \nonumber\end{equation}
\begin{equation} \bm{B}^{2} = \alpha ^{2} {\left ( n_{m} \right )}^{2} {\left ( s_{a} \right )}^{2} {\left ( s_{b} \right )}^{2} + 2 \alpha  c_{a} c_{b} n_{m} s_{a} s_{b} - {\left ( c_{a} \right )}^{2} n_{b} n_{m} {\left ( s_{b} \right )}^{2} - {\left ( c_{b} \right )}^{2} n_{a} n_{m} {\left ( s_{a} \right )}^{2} - n_{a} n_{b} {\left ( n_{m} \right )}^{2} {\left ( s_{a} \right )}^{2} {\left ( s_{b} \right )}^{2} \nonumber\end{equation}
\begin{equation} S^{2}-B^{2} = {\left ( c_{a} \right )}^{2} {\left ( c_{b} \right )}^{2} + {\left ( c_{a} \right )}^{2} n_{b} n_{m} {\left ( s_{b} \right )}^{2} + {\left ( c_{b} \right )}^{2} n_{a} n_{m} {\left ( s_{a} \right )}^{2} + n_{a} n_{b} {\left ( n_{m} \right )}^{2} {\left ( s_{a} \right )}^{2} {\left ( s_{b} \right )}^{2} \nonumber\end{equation}
\begin{equation} S^{2}-B^{2} = {\left ( c_{a} \right )}^{2} {\left ( c_{b} \right )}^{2} + {\left ( c_{a} \right )}^{2} n_{b} n_{m} {\left ( s_{b} \right )}^{2} + {\left ( c_{b} \right )}^{2} n_{a} n_{m} {\left ( s_{a} \right )}^{2} + n_{a} n_{b} {\left ( s_{a} \right )}^{2} {\left ( s_{b} \right )}^{2} \nonumber\end{equation}
\begin{equation} \T{Consider all combinations of} \bm{e}_{a}^{2}, \bm{e}_{b}^{2} \T{and} \bm{e}_{m}^2: \nonumber\end{equation}
\begin{equation} \left [ \bm{e}_{a}^{2},\bm{e}_{b}^{2},\bm{e}_{m}^2\right ] = [-1, -1, -1] \nonumber\end{equation}
\begin{equation} S^{2}-\bm{B}^{2} = {\sin{\left (\theta _{a} \right )}}^{2} {\sin{\left (\theta _{b} \right )}}^{2} + {\sin{\left (\theta _{a} \right )}}^{2} {\cos{\left (\theta _{b} \right )}}^{2} + {\sin{\left (\theta _{b} \right )}}^{2} {\cos{\left (\theta _{a} \right )}}^{2} + {\cos{\left (\theta _{a} \right )}}^{2} {\cos{\left (\theta _{b} \right )}}^{2}  = 1 \nonumber\end{equation}
\begin{equation} \left [ \bm{e}_{a}^{2},\bm{e}_{b}^{2},\bm{e}_{m}^2\right ] = [-1, -1, 1] \nonumber\end{equation}
\begin{equation} S^{2}-\bm{B}^{2} = {\sinh{\left (\theta _{a} \right )}}^{2} {\sinh{\left (\theta _{b} \right )}}^{2} - {\sinh{\left (\theta _{a} \right )}}^{2} {\cosh{\left (\theta _{b} \right )}}^{2} - {\sinh{\left (\theta _{b} \right )}}^{2} {\cosh{\left (\theta _{a} \right )}}^{2} + {\cosh{\left (\theta _{a} \right )}}^{2} {\cosh{\left (\theta _{b} \right )}}^{2}  = 1 \nonumber\end{equation}
\begin{equation} \left [ \bm{e}_{a}^{2},\bm{e}_{b}^{2},\bm{e}_{m}^2\right ] = [-1, 1, -1] \nonumber\end{equation}
\begin{equation} S^{2}-\bm{B}^{2} = - {\sin{\left (\theta _{a} \right )}}^{2} {\sinh{\left (\theta _{b} \right )}}^{2} + {\sin{\left (\theta _{a} \right )}}^{2} {\cosh{\left (\theta _{b} \right )}}^{2} - {\cos{\left (\theta _{a} \right )}}^{2} {\sinh{\left (\theta _{b} \right )}}^{2} + {\cos{\left (\theta _{a} \right )}}^{2} {\cosh{\left (\theta _{b} \right )}}^{2}  = 1 \nonumber\end{equation}
\begin{equation} \left [ \bm{e}_{a}^{2},\bm{e}_{b}^{2},\bm{e}_{m}^2\right ] = [-1, 1, 1] \nonumber\end{equation}
\begin{equation} S^{2}-\bm{B}^{2} = - {\sin{\left (\theta _{b} \right )}}^{2} {\sinh{\left (\theta _{a} \right )}}^{2} + {\sin{\left (\theta _{b} \right )}}^{2} {\cosh{\left (\theta _{a} \right )}}^{2} - {\cos{\left (\theta _{b} \right )}}^{2} {\sinh{\left (\theta _{a} \right )}}^{2} + {\cos{\left (\theta _{b} \right )}}^{2} {\cosh{\left (\theta _{a} \right )}}^{2}  = 1 \nonumber\end{equation}
\begin{equation} \left [ \bm{e}_{a}^{2},\bm{e}_{b}^{2},\bm{e}_{m}^2\right ] = [1, -1, -1] \nonumber\end{equation}
\begin{equation} S^{2}-\bm{B}^{2} = - {\sin{\left (\theta _{b} \right )}}^{2} {\sinh{\left (\theta _{a} \right )}}^{2} + {\sin{\left (\theta _{b} \right )}}^{2} {\cosh{\left (\theta _{a} \right )}}^{2} - {\cos{\left (\theta _{b} \right )}}^{2} {\sinh{\left (\theta _{a} \right )}}^{2} + {\cos{\left (\theta _{b} \right )}}^{2} {\cosh{\left (\theta _{a} \right )}}^{2}  = 1 \nonumber\end{equation}
\begin{equation} \left [ \bm{e}_{a}^{2},\bm{e}_{b}^{2},\bm{e}_{m}^2\right ] = [1, -1, 1] \nonumber\end{equation}
\begin{equation} S^{2}-\bm{B}^{2} = - {\sin{\left (\theta _{a} \right )}}^{2} {\sinh{\left (\theta _{b} \right )}}^{2} + {\sin{\left (\theta _{a} \right )}}^{2} {\cosh{\left (\theta _{b} \right )}}^{2} - {\cos{\left (\theta _{a} \right )}}^{2} {\sinh{\left (\theta _{b} \right )}}^{2} + {\cos{\left (\theta _{a} \right )}}^{2} {\cosh{\left (\theta _{b} \right )}}^{2}  = 1 \nonumber\end{equation}
\begin{equation} \left [ \bm{e}_{a}^{2},\bm{e}_{b}^{2},\bm{e}_{m}^2\right ] = [1, 1, -1] \nonumber\end{equation}
\begin{equation} S^{2}-\bm{B}^{2} = {\sinh{\left (\theta _{a} \right )}}^{2} {\sinh{\left (\theta _{b} \right )}}^{2} - {\sinh{\left (\theta _{a} \right )}}^{2} {\cosh{\left (\theta _{b} \right )}}^{2} - {\sinh{\left (\theta _{b} \right )}}^{2} {\cosh{\left (\theta _{a} \right )}}^{2} + {\cosh{\left (\theta _{a} \right )}}^{2} {\cosh{\left (\theta _{b} \right )}}^{2}  = 1 \nonumber\end{equation}
\begin{equation} \left [ \bm{e}_{a}^{2},\bm{e}_{b}^{2},\bm{e}_{m}^2\right ] = [1, 1, 1] \nonumber\end{equation}
\begin{equation} S^{2}-\bm{B}^{2} = {\sin{\left (\theta _{a} \right )}}^{2} {\sin{\left (\theta _{b} \right )}}^{2} + {\sin{\left (\theta _{a} \right )}}^{2} {\cos{\left (\theta _{b} \right )}}^{2} + {\sin{\left (\theta _{b} \right )}}^{2} {\cos{\left (\theta _{a} \right )}}^{2} + {\cos{\left (\theta _{a} \right )}}^{2} {\cos{\left (\theta _{b} \right )}}^{2}  = 1 \nonumber\end{equation}
\begin{equation} \T{Thus we have shown that }R_{a}R_{b} = S+\bm{D} = e^{\bm{C}} \T{where} \bm{C} \T{is a bivector blade.} \nonumber\end{equation}
\end{document}
